
\section*{Why}

Given $a, b, c$ nonzero real numbers, find $x$ to solve $ax^2 + bx + c = 0$.

\section*{Result}

\begin{proposition}
Let $a, b, c \in \R $ nonzero.
Then both
\[
\frac{-b + \sqrt{b^2 - 4ac}}{2a}
\quad \text{ and } \quad
\frac{-b - \sqrt{b^2 - 4ac}}{2a}
\]
are solutions of
\[
ax^2 + bx + c = 0.
\]
\end{proposition}

We call $ax^2 + bx + c = 0$ a \t{quadratic equation}.\footnote{Future editions will prove via completing the square.}
The solutions are often writen in short hand
\[
x = \frac{-b \pm \sqrt{b^2 - 4ac}}{2a},
\]
which is called the \t{quadratic formula}.

\section*{Proof}

\begin{proposition}
Let $p, q \in \R $ be real numbers.
Suppose $x \in \R $ satisfies the second-degree equation
\[
x^2 + px + q = 0
\]
Then
\[
x \in \set{-\frac{p}{2} + \sqrt{\frac{p^2}{4} - q}, -\frac{p}{2} - \sqrt{\frac{p^2}{4} - q}}
\]
\end{proposition}

\begin{proof}Suppose $x \in \R $ satisfies
\[
x^2 + px + q = 0
\]
This holds if and only if
\[
x^2 + px = -q
\]
which holds if and only if
\[
x^2 + px + \frac{p^2}{4} = \frac{p^2}{4} - q
\]
We can express the left hand side as
\[
x^2 + px + \frac{p^2}{4} = \left(x + \frac{p}{2}\right)^2
\]
By substituting this into the left hand side, we have that $x$ is a solution if and only if
\[
\left(x + \frac{p}{2}\right)^2 = \frac{p^2}{4} - q,
\]
Hence $x$ is a solution if and only if $x + p/2$ is a square root of $p^2/4 - q$.
As usual, there are two quantities, which we denote as usual with $\sqrt{\cdot }$, so that $x$ is a solution if and only if
\[
x + \frac{p}{2} = \pm\sqrt{\frac{p^2}{4} - q}
\]
Consequently, $x$ is a solution if and only if
\[
x = -\frac{p}{2} \pm \sqrt{\frac{p^2}{4} - q}
\]\end{proof}
\begin{corollary}
A real number $x$ satisfies $ax^2 + bx + c = 0$ if and only if $x = \frac{-b \pm \sqrt{b^2-4ac}}{2a}$.
\end{corollary}

\begin{proof}Divide through by $a$.
Define $p = b/a$ and $q = c/a$.
Then we have that $x$ is a solution if and only if
\[
x = -\frac{b}{2a} \pm \sqrt{\frac{b^2}{4a^2} - \frac{c}{a}}
\]
Which holds if and only if
\[
x = \frac{-b}{2a} \pm \sqrt{\frac{b^2}{4a^2} - \frac{4ac}{4a^2}}
\]
which holds if and only if
\[
x = \frac{-b \pm \sqrt{b^2 - 4ac}}{2a},
\]
as desired.\end{proof}