
%!name:independent_event_sigma_algebras
%!need:independent_sigma_algebras

\section*{Definition}

The \t{event sigma algebra} of $A \in \mathcal{F} $ where $(\Omega , \mathcal{F} )$ is a measurable space is the set sub-$\sigma $-algebra $\set{\varnothing, A, A^c, \Omega }$.

A family of events events are \t{independent} if the event sigma algebras are independent.

\subsection*{Notation}

Let $(X, \mathcal{A} , \mu )$ be a probability space.
Let $A \in \mathcal{A} $ be an event.
The sigma algebra generated by $A$ is $\set*{\varnothing, A, X - A, X}$.
We denote it by $\sigma (A)$.

Let $B \in \mathcal{A} $.
If $A$ is independent of $B$ we write $A \perp  B$.

\section*{Equivalent condition}

\begin{proposition}
Two events are independent if and only if the measure of their intersection is the product of their measures.\end{proposition}
\begin{proof}Let $(X, \mathcal{A} , \mu )$ be a probability space.
Let $A, B \in \mathcal{A} $.

$(\Rightarrow)$ If $A \perp  B$, then by definition $A \in \sigma (A)$ and $B \in \sigma (B)$ and so:
    \[
\mu (A \cap  B) = \mu (A)\mu (B).
    \]

$(\Leftarrow)$ Conversely, let $a \in \sigma (A)$ and $b \in \sigma (B)$.
If $a = \varnothing$ or $b = \varnothing$ then $a \cap  b = \varnothing$.
So
    \[
\mu (a \cap  b) = \mu (\varnothing) = \mu (a)\mu (b),
    \]
since one of the two measures on the right hand side is zero.
On the other hand, if $a = X$, then $a \cap  b = b$ and so
    \[
\mu (a \cap  b) = \mu (b) = \mu (a)\mu (b),
    \]
since $\mu (a) = \mu (X) = 1$.
Likewise if $b = X$.

So it remains to verify $\mu (a \cap  b) = \mu (a)\mu (b)$ for the cases $a \in \set{A,X -A}$ and $b \in \set{B, X-B}$.
If $a = A$, and $b = B$, then the identity follows by hypothesis.
Next, observe that $A \cap  (X - B) = A - (A \cap  B)$ and $(A \cap  B) \subset A$ so $\mu (X) < \infty$ allows us to deduce:
    \[
\begin{aligned}
\mu (A \cap  (X - B)) &= \mu (A - (A \cap  B)) \\
&= \mu (A) - \mu (A \cap  B) \\
&= \mu (A)(1 - \mu (B)) \\
&= \mu (A)\mu (X - A).
\end{aligned}
    \]
Similar for $X-A$ and $B$.
Finally, recall that $\mu (A \cup B) = \mu (A) + \mu (B) - \mu (A \cap  B)$.
So then,
    \[
\begin{aligned}
\mu ((X - A) \cap  (X - B)) &= 1 - \mu (A \cup B) \\
&= 1 - \mu (A) - \mu (B) + \mu (A \cap  B) \\
&= 1 - \mu (A) - \mu (B) + \mu (A)\mu (B) \\
&= (1 - \mu (A))(1 - \mu (B)) \\
&= \mu (X - A)\mu (X - B).
\end{aligned}
    \]
\end{proof}