%!name:sigma_algebra_event_independence
%!need:sigma_algebra_independence

\ssection{Why}
  \ifhmode\unskip\fi\footnote{
Future editions will include
  }

\ssection{Definition}

The sigma algebra \t{generated by an event} is the sigma algebra consisting of the empty set, the event, the complement (in the base set) of the event, and the base set.

A family of events events are \t{independent} if the sigma algebras generated by the events are independent.

\ssubsection{Notation}

Let $(X, \SA, \mu )$ be a probability space.
Let $A \in \SA$ be an event.
The sigma algebra generated by $A$ is $\set*{\emptyset, A, X - A, X}$.
We denote it by $\sigma (A)$.

Let $B \in \SA$.
If $A$ is independent of $B$ we write $A \perp B$.

\ssection{Equivalent Condition}

\begin{proposition}
Two events are independent if and only if the measure of their intersection is the product of their measures.

\begin{proof}
Let $(X, \SA, \mu )$ be a probability space.
Let $A, B \in \SA$.

$(\Rightarrow)$ If $A \perp B$, then by definition $A \in \sigma (A)$ and $B \in \sigma (B)$ and so:
  \[
\mu (A \cap B) = \mu (A)\mu (B).
  \]

$(\Leftarrow)$ Conversely, let $a \in \sigma (A)$ and $b \in \sigma (B)$.
If $a = \varnothing$ or $b = \varnothing$ then $a \cap b = \varnothing$.
So
  \[
\mu (a \cap b) = \mu (\varnothing) = \mu (a)\mu (b),
  \]
since one of the two measures on the right hand side is zero.
On the other hand, if $a = X$, then $a \cap b = b$ and so
  \[
\mu (a \cap b) = \mu (b) = \mu (a)\mu (b),
  \]
since $\mu (a) = \mu (X) = 1$.
Likewise if $b = X$.

So it remains to verify $\mu (a \cap b) = \mu (a)\mu (b)$ for the cases $a \in \set{A,X -A}$ and $b \in \set{B, X-B}$.
If $a = A$, and $b = B$, then the identity follows by hypothesis.
Next, observe that $A \cap (X - B) = A - (A \cap B)$ and $(A \cap B) \subset A$ so $\mu (X) < \infty$ allows us to deduce:
  \[
\begin{aligned}
\mu (A \cap (X - B)) &= \mu (A - (A \cap B)) \\
&= \mu (A) - \mu (A \cap B) \\
&= \mu (A)(1 - \mu (B)) \\
&= \mu (A)\mu (X - A).
\end{aligned}
  \]
Similar for $X-A$ and $B$.
Finally, recall that $\mu (A \cup B) = \mu (A) + \mu (B) - \mu (A \cap B)$.
So then,
  \[
\begin{aligned}
\mu ((X - A) \cap (X - B)) &= 1 - \mu (A \cup B) \\
&= 1 - \mu (A) - \mu (B) + \mu (A \cap B) \\
&= 1 - \mu (A) - \mu (B) + \mu (A)\mu (B) \\
&= (1 - \mu (A))(1 - \mu (B)) \\
&= \mu (X - A)\mu (X - B).
\end{aligned}
  \]
\end{proof}
\end{proposition}
